Added SET_NZCV_ID, which goes into PSR_CONV.
Also exported (to ML) the small bit of of the ARM spec that doesn't cause any
problems (i.e. the bits that have nothing to do with words).  Had to rename
the type "interrupt" to "interrupts" because the former obviously doesn't work
in ML.

examples/elliptic/arm/arm_evalLib.sml
@@ -56,8 +56,8 @@ fun arm_compset () = add_rws wordsLib.words_compset
    mode_EQ_mode,mode2num_thm,mode_case_def,
    psrs_EQ_psrs,psrs2num_thm,
    iclass_EQ_iclass,iclass2num_thm,
-   exception_EQ_exception,exception2num_thm,exception_case_def,
-   num2exception_thm,exception2mode_def,
+   exceptions_EQ_exceptions,exceptions2num_thm,exceptions_case_def,
+   num2exceptions_thm,exceptions2mode_def,
    num2condition_thm,condition2num_thm,condition_case_def,
    interrupts_case_def,
    SUBST_EVAL,
@@ -132,7 +132,7 @@ fun arm_compset () = add_rws wordsLib.words_compset
    MLA_MUL_def,SWP_def,MRC_def,MCR_OUT_def,MSR_def,LDM_STM_def,LDC_STC_def,
 
    SIMP_RULE (std_ss++pred_setSimps.PRED_SET_ss) []
-      interrupt2exception_def,
+      interrupt2exceptions_def,
    IS_Dabort_def,IS_Reset_def,PROJ_Dabort_def,PROJ_Reset_def,
    THE_DEF,IS_SOME_DEF,IS_NONE_EQ_NONE,NOT_IS_SOME_EQ_NONE,
    option_case_ID,option_case_SOME_ID,
